coq/Core.v
@@ -42,11 +42,19 @@ Ltac intro_term :=
   | [|- seq (rule _) -> _] => intro
   | [|- exp _ -> _] => intro
   | [|- ctx _ -> _] => intro
-  | [|- seq (ctx_var _) -> _] => intro
-  | [|- ctx_var _ -> _] => intro
+  | [|- seq (exp _) -> _] => intro
   | [|- rule _ -> _] => intro
   | [|- subst _ -> _] => intro
   end.
+
+Tactic Notation "intro_to" constr(ty) :=
+  repeat lazymatch goal with
+         | |- ty -> _ => idtac
+         | |- ty _ -> _ => idtac
+         | |- ty _ _-> _ => idtac
+         | |- ty _ _ _ -> _ => idtac
+         | |- _ -> _ => intro
+         end.
 
 Ltac construct_with t :=
   constructor; apply: t; eauto.
@@ -58,30 +66,24 @@ Ltac solve_wf_with t :=
 
 (* well-formed language suppositions *)
 Lemma wf_ctx_lang  {p} (l : lang p) c (wf : wf_ctx l c) : wf_lang l
-with wf_ctx_var_lang  {p} (l : lang p) c v (wf : wf_ctx_var l c v) : wf_lang l
 with wf_sort_lang  {p} (l : lang p) c t (wf : wf_sort l c t) : wf_lang l.
-  all: case: wf => //=.
-  solve_wf_with wf_ctx_var_lang.
-  solve_wf_with wf_ctx_lang.
-  solve_wf_with wf_sort_lang.
+  all: case: wf => //=;
   solve_wf_with wf_sort_lang.
 Qed.
 Hint Immediate wf_ctx_lang.
-Hint Immediate wf_ctx_var_lang.
 Hint Immediate wf_sort_lang.
 
 Lemma wf_term_lang  {p} (l : lang p) c e t
       (wf : wf_term l c e t) : wf_lang l
 with wf_subst_lang  {p} (l : lang p) c s c'
            (wf : wf_subst l c s c') : wf_lang l.
-  all: case: wf => //=.
-  solve_wf_with wf_term_lang.
+  all: case: wf => //=;
+  try solve_wf_with wf_term_lang.
   repeat intro_term.
   move => wft wfs.
   apply: wf_term_lang; eauto.
-  solve_wf_with (@wf_ctx_lang p).
   solve_wf_with (@wf_sort_lang p).
-  solve_wf_with wf_term_lang.
+  solve_wf_with (@wf_ctx_lang p).
 Qed.
 Hint Immediate wf_term_lang.
 Hint Immediate wf_subst_lang.
@@ -105,24 +107,20 @@ Scheme le_sort_mono_ind := Minimality for le_sort Sort Prop
   with le_subst_mono_ind := Minimality for le_subst Sort Prop
   with le_term_mono_ind := Minimality for le_term Sort Prop
   with le_ctx_mono_ind := Minimality for le_ctx Sort Prop
-  with le_ctx_var_mono_ind := Minimality for le_ctx_var Sort Prop
   with wf_sort_mono_ind := Minimality for wf_sort Sort Prop
   with wf_subst_mono_ind := Minimality for wf_subst Sort Prop
   with wf_term_mono_ind := Minimality for wf_term Sort Prop
-  with wf_ctx_mono_ind := Minimality for wf_ctx Sort Prop
-  with wf_ctx_var_mono_ind := Minimality for wf_ctx_var Sort Prop.
+  with wf_ctx_mono_ind := Minimality for wf_ctx Sort Prop.
 
 Combined Scheme mono_ind from
          le_sort_mono_ind,
          le_subst_mono_ind,
          le_term_mono_ind,
          le_ctx_mono_ind,
-         le_ctx_var_mono_ind,
          wf_sort_mono_ind,
          wf_subst_mono_ind,
          wf_term_mono_ind,
-         wf_ctx_mono_ind,
-         wf_ctx_var_mono_ind.
+         wf_ctx_mono_ind.
 
 Lemma mono {p} r
   : (forall (l : lang p) c1 c2 t1 t2,
@@ -136,13 +134,10 @@ Lemma mono {p} r
            wf_rule l r ->
            le_term (r::l) c1 c2 e1 e2 t1 t2)
     /\ (forall (l : lang p) c1 c2,  le_ctx l c1 c2 -> wf_rule l r ->  le_ctx (r::l) c1 c2)
-    /\ (forall (l : lang p) c1 c2 v1 v2,
-           le_ctx_var l c1 c2 v1 v2 -> wf_rule l r ->  le_ctx_var (r::l) c1 c2 v1 v2)
     /\ (forall (l : lang p) c t, wf_sort l c t -> wf_rule l r -> wf_sort (r::l) c t)
     /\ (forall (l : lang p) c s c', wf_subst l c s c' -> wf_rule l r -> wf_subst (r::l) c s c')
     /\ (forall (l : lang p) c e t,  wf_term l c e t -> wf_rule l r ->  wf_term (r::l) c e t)
-    /\ (forall (l : lang p) c,  wf_ctx l c -> wf_rule l r ->  wf_ctx (r::l) c)
-    /\ (forall (l : lang p) c v,  wf_ctx_var l c v -> wf_rule l r ->  wf_ctx_var (r::l) c v).
+    /\ (forall (l : lang p) c,  wf_ctx l c -> wf_rule l r ->  wf_ctx (r::l) c).
 Proof.
   apply: mono_ind; eauto.  
   intros; apply: le_term_conv; eauto.
@@ -155,14 +150,6 @@ Proof.
   apply mono; auto.
 Qed.
 Hint Resolve le_ctx_mono.
-  
-Lemma le_ctx_var_mono {p} (l : lang p) r c1 c2 v1 v2
-                     (wfv : le_ctx_var l c1 c2 v1 v2)
-     : wf_rule l r -> le_ctx_var (r::l) c1 c2 v1 v2.
-Proof.
-  apply mono; auto.
-Qed.
-Hint Resolve le_ctx_var_mono.
 
 Lemma le_sort_mono {p} (l : lang p) r c1 c2 t1 t2
                   (wfs : le_sort l c1 c2 t1 t2)
@@ -213,13 +200,6 @@ Proof.
   apply mono; auto.
 Qed.
 Hint Resolve wf_ctx_mono.
-
-Lemma wf_ctx_var_mono {p} (l : lang p) r c v
-  : wf_ctx_var l c v -> wf_rule l r -> wf_ctx_var (r::l) c v.
-Proof.
-  apply mono; auto.
-Qed.
-Hint Resolve wf_ctx_var_mono.
 
 Lemma wf_rule_mono {p} (l : lang p) r r'
   : wf_rule l r' -> wf_rule l r -> wf_rule (r::l) r'.
@@ -272,27 +252,16 @@ Lemma ctx_trans p (l : lang p) n
   : (forall c1 c2 c3, n = 2 * size c1 -> le_ctx l c1 c2 -> le_ctx l c2 c3 -> le_ctx l c1 c3)
     /\ (forall c1 c2 c3 v1 v2 v3,
            n = (2 * size c1).+1 ->
-           le_ctx_var l c1 c2 v1 v2 ->
-           le_ctx_var l c2 c3 v2 v3 ->
-           le_ctx_var l c1 c3 v1 v3).
+           le_sort l c1 c2 v1 v2 ->
+           le_sort l c2 c3 v2 v3 ->
+           le_sort l c1 c3 v1 v3).
 Proof.
   move: n.
   apply: nat2_mut_ind.
-  - case; repeat intro_term; repeat top_inversion; auto.
-  - case; repeat intro_term; repeat top_inversion; auto.
-  - move => n IH; repeat intro_term;
-    case;
-    repeat top_inversion;
-    constructor;
-    [ apply: IH
-    | apply: le_sort_trans]; eauto.
-  - move => n IH; repeat intro_term.
-    move => neq.
-    repeat top_inversion; constructor; auto.
-    apply: IH; eauto.
-    move: neq.
-    rewrite -H2 !mul2n doubleS.
-    auto.
+  1,2: case; repeat intro_term; repeat top_inversion; auto.
+  all: move => n IH; repeat intro_term;
+    case => neq;
+    repeat top_inversion; subst; eauto.
 Qed.
 
 Lemma le_ctx_trans p (l : lang p) c1 c2 c3 : le_ctx l c1 c2 -> le_ctx l c2 c3 -> le_ctx l c1 c3.
@@ -301,35 +270,14 @@ Proof.
 Qed.
 Hint Resolve le_ctx_trans.
 
-Lemma le_ctx_var_trans p (l : lang p) c1 c2 c3 v1 v2 v3 :
-  le_ctx_var l c1 c2 v1 v2 -> le_ctx_var l c2 c3 v2 v3 -> le_ctx_var l c1 c3 v1 v3.
-Proof.
-  eapply ctx_trans; eauto.
-Qed.
-Hint Resolve le_ctx_var_trans.
 
-Scheme wf_ctx_var_refl_ind := Minimality for wf_ctx_var Sort Prop
-  with wf_ctx_refl_ind := Minimality for wf_ctx Sort Prop.
-Combined Scheme ctx_refl_ind from wf_ctx_refl_ind, wf_ctx_var_refl_ind.
+Scheme ctx_refl_ind := Minimality for wf_ctx Sort Prop.
 
-Lemma le_refl p 
-  : (forall (l : lang p) (c : ctx p), wf_ctx l c -> le_ctx l c c)
-    /\ (forall (l : lang p) c v, wf_ctx_var l c v -> le_ctx_var l c c v v).
+Lemma le_ctx_refl p : forall (l : lang p) (c : ctx p), wf_ctx l c -> le_ctx l c c.
 Proof.
   eapply ctx_refl_ind; eauto.
 Qed.
-
-Lemma le_ctx_refl p (l : lang p) c : wf_ctx l c -> le_ctx l c c.
-Proof.
-  eapply le_refl.
-Qed.
 Hint Resolve le_ctx_refl.
-
-Lemma le_ctx_var_refl p (l : lang p) c v : wf_ctx_var l c v -> le_ctx_var l c c v v.
-Proof.
-  eapply le_refl.
-Qed.
-Hint Resolve le_ctx_var_refl.
 
 
 (* note: this isn't true in general if I add a freshness condition *)
@@ -351,8 +299,7 @@ Proof.
 Qed.
 
 
-Scheme le_wf_ctx_var_ind := Minimality for le_ctx_var Sort Prop
-  with le_wf_ctx_ind := Minimality for le_ctx Sort Prop
+Scheme le_wf_ctx_ind := Minimality for le_ctx Sort Prop
   with le_wf_sort_ind := Minimality for le_sort Sort Prop
   with le_wf_subst_ind := Minimality for le_subst Sort Prop
   with le_wf_term_ind := Minimality for le_term Sort Prop.
@@ -360,8 +307,7 @@ Combined Scheme le_wf_ind from
          le_wf_sort_ind,
          le_wf_subst_ind,
          le_wf_term_ind,
-         le_wf_ctx_ind,
-         le_wf_ctx_var_ind.
+         le_wf_ctx_ind.
 
 
 Lemma le_wf_l {p}
@@ -371,9 +317,7 @@ Lemma le_wf_l {p}
            le_subst l c1 c2 s1 s2 c1' c2' -> wf_subst l c1 s1 c1')
     /\ (forall (l : lang p) c1 c2 e1 e2 t1 t2,
            le_term l c1 c2 e1 e2 t1 t2 -> wf_term l c1 e1 t1)
-    /\ (forall (l : lang p) c1 c2,  le_ctx l c1 c2 -> wf_ctx l c1)
-    /\ (forall (l : lang p) c1 c2 v1 v2,
-           le_ctx_var l c1 c2 v1 v2 -> wf_ctx_var l c1 v1).
+    /\ (forall (l : lang p) c1 c2,  le_ctx l c1 c2 -> wf_ctx l c1).
 Proof.
   apply: le_wf_ind; eauto; repeat intro_term;
     move => wfl /rule_in_wf rin;
@@ -388,9 +332,7 @@ Lemma le_wf_r {p}
            le_subst l c1 c2 s1 s2 c1' c2' -> wf_subst l c2 s2 c2')
     /\ (forall (l : lang p) c1 c2 e1 e2 t1 t2,
            le_term l c1 c2 e1 e2 t1 t2 -> wf_term l c2 e2 t2)
-    /\ (forall (l : lang p) c1 c2,  le_ctx l c1 c2 -> wf_ctx l c2)
-    /\ (forall (l : lang p) c1 c2 v1 v2,
-           le_ctx_var l c1 c2 v1 v2 -> wf_ctx_var l c2 v2).
+    /\ (forall (l : lang p) c1 c2,  le_ctx l c1 c2 -> wf_ctx l c2).
 Proof.
   apply: le_wf_ind; eauto; repeat intro_term;
     move => wfl /rule_in_wf rin;
@@ -407,17 +349,7 @@ Lemma le_ctx_wf_r  {p} (l : lang p) c1 c2 : le_ctx l c1 c2 -> wf_ctx l c2.
 Proof.
     by eapply le_wf_r.
 Qed.
-Hint Immediate le_ctx_wf_r. 
-Lemma le_ctx_var_wf_l  {p} (l : lang p) c1 c2 v1 v2 : le_ctx_var l c1 c2 v1 v2 -> wf_ctx_var l c1 v1.
-Proof.
-    by eapply le_wf_l.
-Qed.
-Hint Immediate le_ctx_var_wf_l.
-Lemma le_ctx_var_wf_r  {p} (l : lang p) c1 c2 v1 v2 : le_ctx_var l c1 c2 v1 v2 -> wf_ctx_var l c2 v2.
-Proof.
-    by eapply le_wf_r.
-Qed.
-Hint Immediate le_ctx_var_wf_r.
+Hint Immediate le_ctx_wf_r.
 Lemma le_sort_wf_l  {p} (l : lang p) c1 c2 t1 t2 : le_sort l c1 c2 t1 t2 -> wf_sort l c1 t1.
 Proof.
     by eapply le_wf_l.
@@ -486,11 +418,12 @@ Fail Qed.
 (* constructor conversion lemmas *)
 
 Ltac rewrite_constr_eqs :=
-  repeat lazymatch goal with
+  repeat match goal with
   | [ |- _ = _ -> _] => move => ->
   | _ => intro
   end.
 
+(* TODO: useful or no?
 Lemma wf_ctx_iff_variant {p} (l : lang p) c : wf_ctx l c <-> wf_ctx_ l c.
 Proof.
   split;case; rewrite_constr_eqs; by eauto.
@@ -562,163 +495,45 @@ Proof.
 Qed.
 Coercion le_term_from_variant p (l : lang p) c1 c2 e1 e2 t1 t2 :=
   iffRL (le_term_iff_variant l c1 c2 e1 e2 t1 t2).
+*)
 
-(* TODO: from here *)
-(*
-Lemma presupp_ctx {p}
-      : forall (l : lang p) c1 c2
-      
-Lemma wf_sort_ctx {p} (l : lang p) c t
-      (wf : wf_sort l c t) : wf_ctx l c.
+Lemma wf_shift_subst {p} (l : lang p) c c'
+  : wf_ctx l (c' ++ c) -> wf_subst l (c' ++ c) (shift_subst (size c) (size c')) c.
 Proof.
-  all: case: wf => //=.
-  + move => l' c' t' wfl lin.
-    have rwf : wf_rule l' ({| c' |- t'}).
-      by apply: rule_in_wf.
-    by inversion rwf.
-  + move => l' c' s c'' t'' wfsb wfs.
-    (* by apply: wf_subst_ctx. TODO: mutual *)
-    give_up.
-Qed.
-
-Lemma le_ctx_wf_l  {p} (l : lang p) c1 c2 (wf : le_ctx l c1 c2) : wf_ctx l c1
-with le_ctx_var_wf_l  {p} (l : lang p) c1 c2 v1 v2
-                      (wf : le_ctx_var l c1 c2 v1 v2) : wf_ctx_var l c1 v1
-with le_sort_wf_l  {p} (l : lang p) c1 c2 t1 t2
-                   (wf : le_sort l c1 c2 t1 t2) : wf_sort l c1 t1.
-  all: case: wf => //=.
-  solve_wf_with (@wf_ctx_nil p).
-  solve_wf_with le_ctx_var_wf_l.
-  solve_wf_with le_ctx_wf_l.
-  solve_wf_with le_sort_wf_l.
-  - move => l' c1' c2' t1' t2' wfl lin.
-    apply List.in_split in lin;
-      case: lin => ll;
-      case => lr l'eq.
-    rewrite l'eq in wfl.
-    pose wfl' := (wf_lang_prefix wfl).
-    inversion wfl'.
-    inversion H0.
-    rewrite l'eq.
-    move: l'eq wfl' => _ _.
-    elim: ll wfl H8; simpl; auto.
-    move => r' ll IH wfl' wfs.
-    apply: wf_sort_mono; auto.
-    apply: IH; auto.
-    inversion wfl'.
-    apply: wf_rule_lang; eauto.
-    inversion wfl'; auto.
-  - move => l' c1' c2' s1 s2 c1'' c2'' t1' t2' lesb les.
-    apply: le_sort_wf_l.
+  elim: c c'.
+  - move => c';
+    rewrite cats0;
+      simpl;
+      auto.
+  - intros.
+    simpl.
+    constructor;
+    move: H0;
+      change (a :: l0) with ([::a]++ l0);
+      suff: size (c'++[::a]) = (size c').+1;
+      try (by elim: c'; simpl; auto);
+      move <-.
+    + rewrite catA;
+        by apply H.
+    + move=> wfc.
+      rewrite extract_var_shift.
+      erewrite <-shift_subst_shift.
+      instantiate(1:=1).
+      (*TODO: strengthen? e.g. n <= size c'?*)
+      eapply wf_term_subst.
+      change (size c') with (0+(size c')).
+      erewrite <-lookup_in_shift_subst; eauto.
+      eapply wf_term_subst.
+ 
     
-    Check List.in_split.
-  Search _ (List.In).
-  (* depends on monotonicity *)
-Qed.
-*)
-
-
-(* =======================
-   OLD: update to work with present definition
-===============================*)
-
-(*
-
-(* well-formed context suppositions *)
-Lemma wf_sort_ctx  {p} (l : lang p) c1 c2 t1 t2
-           (wf : wf_sort l c1 c2 t1 t2) : wf_ctx l c1 c2.
-  case: wf => //=.
-Qed.
-Hint Immediate wf_sort_ctx : wf_hints.
-Lemma wf_ctx_var_ctx  {p} (l : lang p) c1 c2 v1 v2
-           (wf : wf_ctx_var l c1 c2 v1 v2) : wf_ctx l c1 c2.
-  case: wf => //= l' c1' c2' t1 t2 _ /wf_sort_ctx //=.
-Qed.
-Hint Immediate wf_ctx_var_ctx : wf_hints.
-Lemma wf_term_ctx  {p} (l : lang p) c1 c2 e1 e2 t1 t2
-           (wf : wf_term l c1 c2 e1 e2 t1 t2) : wf_ctx l c1 c2.
-  case: wf => //=.
-Qed.
-Hint Immediate wf_term_ctx : wf_hints.
-Lemma wf_subst_ctx  {p} (l : lang p) c1 c2 s1 s2 c1' c2'
-           (wf : wf_subst l c1 c2 s1 s2 c1' c2') : wf_ctx l c1 c2.
-  case: wf => //=.
-Qed.
-Hint Immediate wf_subst_ctx : wf_hints.
-Lemma wf_subst_ctx_out  {p} (l : lang p) c1 c2 s1 s2 c1' c2'
-           (wf : wf_subst l c1 c2 s1 s2 c1' c2') : wf_ctx l c1' c2'.
-  case: wf => //=.
-Qed.
-Hint Immediate wf_subst_ctx_out : wf_hints.
-
-(* well-formed sort presuppositions *)
-Lemma wf_term_sort {p} (l : lang p) c1 c2 e1 e2 t1 t2
-           (wf : wf_term l c1 c2 e1 e2 t1 t2) : wf_sort l c1 c2 t1 t2.
-  case: wf => //=.
-Qed.
-Hint Immediate wf_term_sort : wf_hints.
-
-
-Lemma wf_sort_conv {p} (l : lang p) c t : wf_sort l c t <-> wf_sort_ l c t.
+    
+Lemma wf_sort_weaken {p} (l : lang p) c s
+  : wf_sort l c s -> forall v, wf_ctx_var l c v -> wf_sort l (v::c) s^!1.
 Proof.
-  split; case; auto.
-  - constructor.
-    TODO
-
-TODO: place these tactics well wrt wf_..._convs
-Ltac hypothesize :=
-  try match goal with
-        [|- _ -> _] => let H := fresh in move => H; hypothesize
-      end.
-
-Ltac solve_wf_lang :=
-  match goal with
-  | [H : wf_ctx ?l _ _ |- wf_lang ?l] => apply: wf_ctx_lang; exact H
-  | [H : wf_ctx_var ?l _ _ _ _ |- wf_lang ?l] => apply: wf_ctx_var_lang; exact H
-  | [H : wf_sort ?l _ _ _ _ |- wf_lang ?l] => apply: wf_sort_lang; exact H
-  | [H : wf_term ?l _ _ _ _ _ _ |- wf_lang ?l] => apply: wf_term_lang; exact H
-  | [H : wf_subst ?l _ _ _ _ _ _ |- wf_lang ?l] => apply: wf_subst_lang; exact H
-  | [H : wf_rule ?l _ |- wf_lang ?l] => apply: wf_rule_lang; exact H
-  end.
-
-Ltac solve_wf_ctx :=
-  match goal with
-  | [H : wf_ctx_var ?l ?c1 ?c2 _ _ |- wf_ctx ?l ?c1 ?c2] => apply: wf_ctx_var_ctx; exact H
-  | [H : wf_sort ?l ?c1 ?c2 _ _ |- wf_ctx ?l ?c1 ?c2] => apply: wf_sort_ctx; exact H
-  | [H : wf_term ?l ?c1 ?c2 _ _ _ _ |- wf_ctx ?l ?c1 ?c2] => apply: wf_term_ctx; exact H
-  | [H : wf_subst ?l ?c1 ?c2 _ _ _ _ |- wf_ctx ?l ?c1 ?c2] => apply: wf_subst_ctx; exact H
-  | [H : wf_subst ?l _ _ _ _ ?c1 ?c2 |- wf_ctx ?l ?c1 ?c2] => apply: wf_subst_ctx_out; exact H
-  end.
-
-Ltac constr_wf :=
-  apply: wf_sort_by
-    + apply: wf_sort_trans
-    + apply: wf_ctx_nil
-    + apply: wf_ctx_cons
-    + apply: wf_sort_var
-    + apply: wf_term_var
-    + apply: wf_term_by
-    + apply: wf_term_trans
-    + apply: wf_term_conv_l
-    + apply: wf_term_conv_r
-    (* good variants *)
-    + apply: wf_ctx_nil_
-    + apply: wf_ctx_cons_
-    + apply: wf_sort_by_
-    + apply: wf_sort_trans_
-    + apply: wf_sort_var_
-    + apply: wf_term_var_
-    + apply: wf_term_by_
-    + apply: wf_term_trans_
-    + apply: wf_term_conv_l_
-    + apply: wf_term_conv_r_
-             + idtac. 
+  intros.
+  suff: ws_exp (size c) s => [wse|].
+  erewrite <-shift_subst_shift; eauto.
+  apply: wf_sort_subst; eauto.
+  give_up. (* need to prove that shift_substs are well-typed *)
+  give_up. (* need to prove that well-typed terms are well-scoped*)
   
-Ltac solve_wf :=
-  by hypothesize;
-  constr_wf;
-  do [solve_wf_lang
-     | solve_wf_ctx
-     | eauto].
-  
-*)
