coq/CoreDefs.v
@@ -57,6 +57,9 @@ with wf_term {p} : lang p -> ctx p -> exp p -> exp p -> Prop :=
     wf_term l c e t ->
     le_sort l c c' t t' ->
     wf_term l c' e t'
+| wf_term_var : forall l c t,
+    wf_sort l c t ->
+    wf_term l (t :: c) (var 0) t
 with le_term {p} : lang p ->
                    ctx p -> ctx p ->
                    exp p -> exp p ->
@@ -93,14 +96,10 @@ with wf_subst {p} : lang p -> ctx p -> subst p ->  ctx p -> Prop :=
 | wf_subst_nil : forall l c,
     wf_ctx l c ->
     wf_subst l c [::] [::]
-| wf_subst_sort : forall l c s c' t,
-    wf_subst l c s c' ->
-    wf_sort l c t ->
-    wf_subst l c (t::s) (sort_var :: c')
-| wf_subst_term : forall l c s c' e t,
+| wf_subst_cons : forall l c s c' e t,
     wf_subst l c s c' ->
     wf_term l c e t[/s/] ->
-    wf_subst l c (e::s) (term_var t::c')
+    wf_subst l c (e::s) (t::c')
 with le_subst {p} : lang p ->
                     ctx p -> ctx p ->
                     subst p -> subst p ->
@@ -108,37 +107,19 @@ with le_subst {p} : lang p ->
 | le_subst_nil : forall l c1 c2,
     le_ctx l c1 c2 ->
     le_subst l c1 c2 [::] [::] [::] [::]
-| le_subst_sort : forall l c1 c2 s1 s2 c1' c2' t1 t2,
-    le_subst l c1 c2 s1 s2 c1' c2' ->
-    le_sort l c1 c2 t1 t2 ->
-    le_subst l c1 c2 (t1::s1) (t2::s2) (sort_var::c1') (sort_var::c2')
-| le_subst_term : forall l c1 c2 s1 s2 c1' c2' e1 e2 t1 t2,
+| le_subst_cons : forall l c1 c2 s1 s2 c1' c2' e1 e2 t1 t2,
     le_subst l c1 c2 s1 s2 c1' c2' ->
     le_term l c1 c2 e1 e2 t1[/s1/] t2[/s2/] ->
-    le_subst l c1 c2 (e1::s1) (e2::s2) (term_var t1::c1') (term_var t2 :: c2')
-with wf_ctx_var {p} : lang p -> ctx p -> ctx_var p -> Prop :=
-| wf_sort_var : forall l c,
-    wf_ctx l c ->
-    wf_ctx_var l c sort_var
-| wf_term_var : forall l c t,
-    wf_sort l c t ->
-    wf_ctx_var l c (term_var t)
-with le_ctx_var {p} : lang p -> ctx p -> ctx p -> ctx_var p -> ctx_var p -> Prop :=
-| le_sort_var : forall l c1 c2,
-    le_ctx l c1 c2 ->
-    le_ctx_var l c1 c2 sort_var sort_var
-| le_term_var : forall l c1 c2 t1 t2,
-    le_sort l c1 c2 t1 t2 ->
-    le_ctx_var l c1 c2 (term_var t1) (term_var t2)
+    le_subst l c1 c2 (e1::s1) (e2::s2) (t1::c1') (t2 :: c2')
 with wf_ctx {p} : lang p -> ctx p -> Prop :=
 | wf_ctx_nil : forall l, wf_lang l -> wf_ctx l [::]
 | wf_ctx_cons : forall l c v,
-    wf_ctx_var l c v ->
+    wf_sort l c v ->
     wf_ctx l (v::c)
 with le_ctx {p} : lang p -> ctx p -> ctx p -> Prop :=
 | le_ctx_nil : forall l, wf_lang l -> le_ctx l [::] [::]
 | le_ctx_cons : forall l c1 c2 v1 v2,
-    le_ctx_var l c1 c2 v1 v2 ->
+    le_sort l c1 c2 v1 v2 ->
     le_ctx l (v1::c1) (v2::c2)
 with wf_rule {p} : lang p -> rule p -> Prop :=
 | wf_sort_rule : forall l c t,
@@ -169,8 +150,6 @@ Hint Constructors wf_term.
 Hint Constructors le_term.
 Hint Constructors wf_subst.
 Hint Constructors le_subst.
-Hint Constructors wf_ctx_var.
-Hint Constructors le_ctx_var.
 Hint Constructors wf_ctx.
 Hint Constructors le_ctx.
 Hint Constructors wf_rule.
@@ -216,6 +195,8 @@ These can't all be mutually inductive since they have different parameters,
 so they are just defined by reference to the core datatypes
  *)
 
+(*
+(*TODO: out of date wrt vars. Are these really worth it? *)
 Variant wf_sort_ {p} (l : lang p) c t : Prop :=
 | wf_sort_by_ :  wf_lang l ->  List.In ({| c|- t})%rule l -> wf_sort_ l c t
 | wf_sort_subst_ : forall s c' t',
@@ -325,8 +306,8 @@ Variant le_subst_ {p} (l : lang p) c1 c2
 Hint Constructors le_subst_.
 
 Variant wf_ctx_var_ {p} (l : lang p) c : ctx_var p -> Prop :=
-| wf_sort_var_ :  wf_ctx l c ->  wf_ctx_var_ l c sort_var
-| wf_term_var_ : forall t, wf_sort l c t -> wf_ctx_var_ l c (term_var t).
+| wf_ctx_var_sort_ :  wf_ctx l c ->  wf_ctx_var_ l c sort_var
+| wf_ctx_var_term_ : forall t, wf_sort l c t -> wf_ctx_var_ l c (term_var t).
 Hint Constructors wf_ctx_var_.
 
 Variant le_ctx_var_ {p} (l : lang p) c1 c2 : ctx_var p -> ctx_var p -> Prop :=
@@ -371,5 +352,5 @@ Variant wf_rule_ {p} (l : lang p) : rule p -> Prop :=
     wf_term_ l c2 e2 t2 ->
     wf_rule_ l ({< c1 <# c2 |- e1 <# e2 .: t1 <# t2}).
 Hint Constructors wf_rule_.
-
+*)
 
